\section*{Task 3}
For r.v. $W$ (taking values in $\Omega$) that represents the environment, we have the generalised belief update equation
\begin{align*}
    \mathcal{P}_W^{t + 1}(w) = \dfrac{\mathcal{P}_W^{t}(w)\mathbb{P}(e_{t+1} | w)}{\int_\Omega\mathcal{P}_W^{t}(\lambda)\mathbb{P}(e_{t+1} | \lambda)\dd\lambda}
\end{align*}

Let $p$ denote fault probability. In this case, $W$ is the (unknown) expected nonfaulty reward of a particular bandit arm and $\Omega=[0,1]$.
\begin{align*}
    \mathbb{P}(e_{t + 1} | w) &= \begin{cases}
        (1-p)w + p\left(\tfrac{1}{2}\cdot 1 + \tfrac{1}{2}\cdot 0\right) & e_{t+1} = 1 \\
        (1-p)(1 - w) + p\left(\tfrac{1}{2}\cdot 0 + \tfrac{1}{2}\cdot 1\right) & e_{t+1} = 0
    \end{cases} \\
    \mathbb{P}(e_{t + 1} | w) &= \begin{cases}
        (1-p)w + \tfrac{p}{2} & e_{t+1} = 1 \\
        1 - \left((1-p)w + \tfrac{p}{2}\right) & e_{t+1} = 0
    \end{cases}
\end{align*}

Thus, writing $w'(w) = (1-p)w + \tfrac{p}{2}$, the belief update equation becomes

\begin{align*}
    \mathcal{P}_W^{t + 1}(w) = \dfrac{\mathcal{P}_W^t(w)(1 - e_{t+1} + (-1)^{1 - e_{t+1}}w'(w))}{\int_\Omega\mathcal{P}_W^t(\lambda)(1 - e_{t+1} + (-1)^{1 - e_{t+1}}w'(\lambda))\dd\lambda}
\end{align*}

Thus, as in the case of classical Thompson sampling, we observe that
\begin{align*}
    \mathcal{P}_W^t(w) &= \begin{cases}
        \mathcal{N}\beta_{s_t+1,f_t+1}\left((1-p)w + \tfrac{p}{2}\right) & w\in[0,1] \\
        0 & \text{otherwise}
    \end{cases}
\end{align*}
where $\mathcal{N}$ is the normalising factor.

The expected faulty reward for arm $a$ is $W'=(1-p)W+\tfrac{p}{2}$, with CDF
\begin{align*}
    f_{W'}^t(x) &= \mathbb{P}\left((1-p)W+\tfrac{p}{2} \leq x\right) \\
    &= \mathbb{P}\left(W \leq \tfrac{2x - p}{2(1 - p)}\right) \\
    &= f_W^t\left(\tfrac{2x - p}{2(1 - p)}\right) \\
    \mathcal{P}_{W'}^t(x) &= \tfrac{1}{1 - p}\mathcal{P}_W^t\left(\tfrac{2x - p}{2(1 - p)}\right) \\
    \Aboxed{\mathcal{P}_{W'}^t(x) &= {\begin{cases}
        \tfrac{\mathcal{N}}{1 - p}\beta_{s_t+1, f_t+1}(x) & x\in\left[\tfrac{p}{2},1-\tfrac{p}{2}\right] \\
        0 & \text{otherwise}
    \end{cases}}}
\end{align*}

Thus for each arm we sample from $\mathcal{B}(s_t+1, f_t+1)$ until we end up in $\left[\tfrac{p}{2},1-\tfrac{p}{2}\right]$, and we pull the arm with the maximum draw.
